thm/abs1_comb_hold_ref_rel_WR_UPScript.sml
@@ -1,0 +1,20 @@
+open HolKernel bossLib boolLib Parse;
+open SPI_stateTheory SPI_relationTheory;
+open driver_stateTheory driver_relationTheory;
+open ds_abs1_stateTheory ds_abs1_relTheory ds_abs1_initTheory ds_abs1_txTheory 
+ds_abs1_rxTheory ds_abs1_xferTheory;
+open ref_relTheory;
+
+val _ = new_theory "abs1_comb_hold_ref_rel_WR_UP";
+
+
+(* simulation: ds_abs1' exists and holds the ref_rel when driver_tau *)
+val abs1_comb_hold_ref_rel_WR_UP = store_thm("abs1_comb_hold_ref_rel_WR_UP",
+``!(spi:spi_state) (dr:driver_state) (ds_abs1:ds_abs1_state).
+(ref_rel ds_abs1 dr spi) /\ (driver_tr dr (Write a v) dr') /\ 
+(spi_tr spi (Update a v) spi') ==>
+(ref_rel ds_abs1 dr' spi') \/
+(?ds_abs1'. (ds_abs1_tr ds_abs1 tau ds_abs1') /\ (ref_rel ds_abs1' dr' spi'))``,
+cheat);
+
+val _ = export_theory();
