thm/abs1_comb_hold_ref_rel_dr_trScript.sml
@@ -4,78 +4,293 @@ open SPI_stateTheory SPI_relationTheory;
 open driver_stateTheory driver_relationTheory driver_checkTheory;
 open ds_abs1_stateTheory ds_abs1_relTheory ds_abs1_initTheory ds_abs1_txTheory 
 ds_abs1_rxTheory ds_abs1_xferTheory;
-open ref_relTheory;
+open ref_relTheory board_memTheory;
 
+val _ = new_theory "abs1_comb_hold_ref_rel_dr_tr";
 
-val _ = new_theory "abs1_comb_hold_ref_rel_spi_tr";
-
-val ref_rel_check_SYSSTATUS = store_thm("ref_rel_check_SYSSTATUS",
-``!(spi:spi_state) (dr:driver_state) (ds_abs1:ds_abs1_state).
+(* driver tau transition to check the SYSSTATUS register *)
+val ref_rel_check_sysstatus = store_thm("ref_rel_check_sysstatus",
+``!(spi:spi_state) (dr:driver_state) (ds_abs1:ds_abs1_state) (v:word32).
 (ref_rel ds_abs1 dr spi) /\ (dr.dr_last_read_ad = SOME SPI0_SYSSTATUS) /\
-(dr.dr_last_read_v = SOME v) /\ (INIT_CHECK_ENABLE dr) ==>
+(dr.dr_last_read_v = SOME v) /\ (dr.state = dr_init_check_rep) ==>
 ref_rel ds_abs1 (dr_check_sysstatus dr v) spi``,
-rw [dr_check_sysstatus_def, INIT_CHECK_ENABLE_def] >|
-[FULL_SIMP_TAC std_ss [ref_rel_def] >>
+rw [dr_check_sysstatus_def] >|
+[FULL_SIMP_TAC std_ss [ref_rel_def, IS_STATE_REL_def] >>
 rw [] >>
-FULL_SIMP_TAC std_ss [IS_INIT_REL_def, IS_TX_REL_def, IS_RX_REL_def, IS_XFER_REL_def] >>
-rw [] >>
-Cases_on `spi.init.state` >>
+Cases_on `spi.state` >>
 rw [] >>
 FULL_SIMP_TAC (std_ss++WORD_ss) [],
-FULL_SIMP_TAC std_ss [ref_rel_def] >>
-rw [] >>
-FULL_SIMP_TAC std_ss [IS_INIT_REL_def, IS_TX_REL_def, IS_RX_REL_def, IS_XFER_REL_def] >>
+FULL_SIMP_TAC std_ss [ref_rel_def, IS_STATE_REL_def] >>
 rw []]);
 
-val ref_rel_check_CH0STAT_TX = store_thm("ref_rel_check_CH0STAT_TX",
+(* driver tau transition to check TXS Bit for tx automaton *)
+val ref_rel_check_tx_txs = store_thm("ref_rel_check_tx_txs",
+``!(spi:spi_state) (dr:driver_state) (ds_abs1:ds_abs1_state) (v:word32).
+(ref_rel ds_abs1 dr spi) /\ (dr.dr_last_read_ad = SOME SPI0_CH0STAT) /\
+(dr.dr_last_read_v = SOME v) /\ (dr.state = dr_tx_check_txs) ==>
+(ref_rel ds_abs1 (dr_check_tx_ch0stat dr v) spi)``,
+rw [dr_check_tx_ch0stat_def] >|
+[FULL_SIMP_TAC std_ss [ref_rel_def, IS_STATE_REL_def] >>
+rw [] >>
+Cases_on `spi.state` >>
+rw [] >> 
+FULL_SIMP_TAC (std_ss++WORD_ss) [],
+FULL_SIMP_TAC std_ss [ref_rel_def, IS_STATE_REL_def] >>
+rw [],
+Cases_on `(1 >< 1) v: word1` >>
+FULL_SIMP_TAC (arith_ss ++ WORD_ss) [] >>
+Cases_on `n` >>
+FULL_SIMP_TAC (arith_ss++WORD_ss) [] >>
+Cases_on `n'` >>
+FULL_SIMP_TAC (arith_ss++WORD_ss) []]);
+
+(* driver tau transition to check EOT Bit for tx automaton *)
+val ref_rel_check_tx_eot = store_thm("ref_rel_check_tx_eot",
+``!(spi:spi_state) (dr:driver_state) (ds_abs1:ds_abs1_state) (v:word32).
+(ref_rel ds_abs1 dr spi) /\ (dr.dr_last_read_ad = SOME SPI0_CH0STAT) /\
+(dr.dr_last_read_v = SOME v) /\ (dr.state = dr_tx_check_eot) ==>
+(ref_rel ds_abs1 (dr_check_tx_ch0stat dr v) spi)``,
+rw [dr_check_tx_ch0stat_def] >|
+[FULL_SIMP_TAC std_ss [ref_rel_def, IS_STATE_REL_def] >>
+rw [] >>
+Cases_on `spi.state` >>
+rw [] >> 
+FULL_SIMP_TAC (std_ss++WORD_ss) [],
+FULL_SIMP_TAC std_ss [ref_rel_def, IS_STATE_REL_def] >>
+rw [],
+Cases_on `(2 >< 2) v: word1` >>
+FULL_SIMP_TAC (arith_ss ++ WORD_ss) [] >>
+Cases_on `n` >>
+FULL_SIMP_TAC (arith_ss++WORD_ss) [] >>
+Cases_on `n'` >>
+FULL_SIMP_TAC (arith_ss++WORD_ss) []]);
+
+(* driver tau transition to check RXS Bit for rx automaton *)
+val ref_rel_check_rx_rxs = store_thm("ref_rel_check_rx_rxs",
+``!(spi:spi_state) (dr:driver_state) (ds_abs1:ds_abs1_state) (v:word32).
+(ref_rel ds_abs1 dr spi) /\ (dr.dr_last_read_ad = SOME SPI0_CH0STAT) /\
+(dr.dr_last_read_v = SOME v) /\ (dr.state = dr_rx_check_rxs) ==>
+(ref_rel ds_abs1 (dr_check_rx_ch0stat dr v) spi)``,
+rw [dr_check_rx_ch0stat_def] >|
+[FULL_SIMP_TAC std_ss [ref_rel_def, IS_STATE_REL_def] >>
+rw [] >>
+Cases_on `spi.state` >>
+rw [] >> 
+FULL_SIMP_TAC (std_ss++WORD_ss) [],
+FULL_SIMP_TAC std_ss [ref_rel_def, IS_STATE_REL_def] >>
+rw []]);
+
+(* lemma:dr.state = dr_rx_fetch_data -> 
+   ds_abs1 is able to perform tau_driver operations, according to ref_rel *)
+val dr_rx_fetch_data_imply_driver_abs1_rx_enable = 
+store_thm ("dr_rx_fetch_data_imply_driver_abs1_rx_enable",
+``!(spi:spi_state) (dr:driver_state) (ds_abs1:ds_abs1_state).
+(ref_rel ds_abs1 dr spi) /\ (dr.state = dr_rx_fetch_data) ==>
+DRIVER_ABS1_RX_ENABLE ds_abs1``,
+rw [DRIVER_ABS1_RX_ENABLE_def] >>
+`IS_STATE_REL ds_abs1 dr spi` by METIS_TAC [ref_rel_def] >>
+FULL_SIMP_TAC std_ss [IS_STATE_REL_def] >>
+Cases_on `spi.state` >>
+rw [] >>
+`(dr.state <> dr_init_pre) /\
+(dr.state <> dr_init_idle) /\
+(dr.state <> dr_init_read_req) /\
+(dr.state <> dr_init_check_rep) /\
+(dr.state <> dr_init_setting) /\
+(dr.state <> dr_ready) /\
+(dr.state <> dr_tx_idle) /\
+(dr.state <> dr_tx_conf_issued) /\
+(dr.state <> dr_tx_read_txs) /\
+(dr.state <> dr_tx_check_txs) /\
+(dr.state <> dr_tx_write_data) /\
+(dr.state <> dr_tx_read_eot) /\
+(dr.state <> dr_tx_check_eot) /\
+(dr.state <> dr_tx_issue_disable) /\
+(dr.state <> dr_tx_reset_conf) /\
+(dr.state <> dr_rx_idle) /\
+(dr.state <> dr_rx_conf_issued) /\
+(dr.state <> dr_rx_read_rxs) /\
+(dr.state <> dr_rx_check_rxs) /\
+(dr.state <> dr_rx_read_rx0) /\
+(dr.state <> dr_rx_issue_disable) /\
+(dr.state <> dr_rx_reset_conf) /\
+(dr.state <> dr_xfer_idle) /\
+(dr.state <> dr_xfer_conf_issued) /\
+(dr.state <> dr_xfer_read_txs) /\
+(dr.state <> dr_xfer_check_txs) /\
+(dr.state <> dr_xfer_write_dataO) /\
+(dr.state <> dr_xfer_read_rxs) /\
+(dr.state <> dr_xfer_check_rxs) /\
+(dr.state <> dr_xfer_read_rx0) /\
+(dr.state <> dr_xfer_fetch_dataI) /\
+(dr.state <> dr_xfer_issue_disable) /\
+(dr.state <> dr_xfer_reset_conf)` by rw [] >>
+Cases_on `ds_abs1.state` >>
+rw []);
+
+(* driver tau transition to check RX0 register for rx automaton *)
+val ref_rel_check_rx_rx0 = store_thm("ref_rel_check_rx_rx0",
+``!(spi:spi_state) (dr:driver_state) (ds_abs1:ds_abs1_state) (v:word32).
+(ref_rel ds_abs1 dr spi) /\ (dr.dr_last_read_ad = SOME SPI0_RX0) /\
+(dr.dr_last_read_v = SOME v) /\ (dr.state = dr_rx_fetch_data) ==>
+?ds_abs1'. (ds_abs1_tr ds_abs1 tau ds_abs1') /\
+(ref_rel ds_abs1' (dr_check_rx0 dr v) spi)``,
+rw [ds_abs1_tr_cases, ds_abs1_dr_tr_cases] >>
+EXISTS_TAC ``driver_abs1_rx_operations ds_abs1`` >>
+`DRIVER_ABS1_RX_ENABLE ds_abs1` by METIS_TAC [dr_rx_fetch_data_imply_driver_abs1_rx_enable] >>
+FULL_SIMP_TAC std_ss [DRIVER_ABS1_RX_ENABLE_def] >>
+rw [dr_check_rx0_def, driver_abs1_rx_operations_def] >|
+[(* abs1_rx_fetch_data, left_length > 1 *)
+`ds_abs1.ds_abs1_rx.rx_left_length > 1` by METIS_TAC [ref_rel_def] >>
+rw [driver_abs1_rx_fetch_data_op_def] >>
+FULL_SIMP_TAC (std_ss++WORD_ss) [ref_rel_def, IS_STATE_REL_def] >>
+rw [],
+(* abs1_rx_fetch_data, left_length = 1 *)
+`~ (ds_abs1.ds_abs1_rx.rx_left_length > 1)` by METIS_TAC [ref_rel_def] >>
+rw [driver_abs1_rx_fetch_data_op_def] >>
+FULL_SIMP_TAC (std_ss++WORD_ss) [ref_rel_def, IS_STATE_REL_def] >>
+rw [],
+(* abs1_rx_next, left_length > 1 *)
+`ds_abs1.ds_abs1_rx.rx_left_length > 1` by METIS_TAC [ref_rel_def] >>
+rw [driver_abs1_rx_next_op_def] >>
+FULL_SIMP_TAC (std_ss++WORD_ss) [ref_rel_def, IS_STATE_REL_def] >>
+rw [],
+(* abs1_rx_next, left_length = 1 *)
+`~ (ds_abs1.ds_abs1_rx.rx_left_length > 1)` by METIS_TAC [ref_rel_def] >>
+rw [driver_abs1_rx_next_op_def] >>
+FULL_SIMP_TAC (std_ss++WORD_ss) [ref_rel_def, IS_STATE_REL_def] >>
+rw [],
+(* abs1_rx_next_ready, left_length > 1 *)
+`ds_abs1.ds_abs1_rx.rx_left_length > 1` by METIS_TAC [ref_rel_def] >>
+rw [driver_abs1_rx_next_ready_op_def] >>
+FULL_SIMP_TAC (std_ss++WORD_ss) [ref_rel_def, IS_STATE_REL_def] >>
+rw [],
+`~ (ds_abs1.ds_abs1_rx.rx_left_length > 1)` by METIS_TAC [ref_rel_def] >>
+rw [driver_abs1_rx_next_ready_op_def] >>
+FULL_SIMP_TAC (std_ss++WORD_ss) [ref_rel_def, IS_STATE_REL_def] >>
+rw []]);
+
+
+val ref_rel_check_xfer_txs = store_thm("ref_rel_check_xfer_txs",
 ``!(spi:spi_state) (dr:driver_state) (ds_abs1:ds_abs1_state).
 (ref_rel ds_abs1 dr spi) /\ (dr.dr_last_read_ad = SOME SPI0_CH0STAT) /\
-(dr.dr_last_read_v = SOME v) /\ (TX_CHECK_ENABLE dr) ==>
-(ref_rel ds_abs1 (dr_check_ch0stat dr v) spi)``,
-rw [TX_CHECK_ENABLE_def, dr_check_ch0stat_def] >|
-[rw [dr_check_tx_ch0stat_def] >|
-[FULL_SIMP_TAC std_ss [ref_rel_def] >>
+(dr.dr_last_read_v = SOME v) /\ (dr.state = dr_xfer_check_txs) ==>
+(ref_rel ds_abs1 (dr_check_xfer_ch0stat dr v) spi)``,
+rw [dr_check_xfer_ch0stat_def] >|
+[FULL_SIMP_TAC std_ss [ref_rel_def, IS_STATE_REL_def] >>
 rw [] >>
-FULL_SIMP_TAC std_ss [IS_INIT_REL_def, IS_TX_REL_def, IS_RX_REL_def, IS_XFER_REL_def] >>
-rw [] >>
-cheat,
-FULL_SIMP_TAC std_ss [ref_rel_def] >>
-rw [] >>
-FULL_SIMP_TAC std_ss [IS_INIT_REL_def, IS_TX_REL_def, IS_RX_REL_def, IS_XFER_REL_def] >>
-rw []],
+Cases_on `spi.state` >>
+rw [] >> 
+FULL_SIMP_TAC (std_ss++WORD_ss) [],
+FULL_SIMP_TAC std_ss [ref_rel_def, IS_STATE_REL_def] >>
+rw [],
+Cases_on `(1 >< 1) v: word1` >>
+FULL_SIMP_TAC (arith_ss ++ WORD_ss) [] >>
+Cases_on `n` >>
+FULL_SIMP_TAC (arith_ss++WORD_ss) [] >>
+Cases_on `n'` >>
+FULL_SIMP_TAC (arith_ss++WORD_ss) []]);
 
-rw [dr_check_tx_ch0stat_def] >|
-[FULL_SIMP_TAC std_ss [ref_rel_def] >>
+val ref_rel_check_xfer_rxs = store_thm("ref_rel_check_xfer_rxs",
+``!(spi:spi_state) (dr:driver_state) (ds_abs1:ds_abs1_state).
+(ref_rel ds_abs1 dr spi) /\ (dr.dr_last_read_ad = SOME SPI0_CH0STAT) /\
+(dr.dr_last_read_v = SOME v) /\ (dr.state = dr_xfer_check_rxs) ==>
+(ref_rel ds_abs1 (dr_check_xfer_ch0stat dr v) spi)``,
+rw [dr_check_xfer_ch0stat_def] >|
+[FULL_SIMP_TAC std_ss [ref_rel_def, IS_STATE_REL_def] >>
 rw [] >>
-FULL_SIMP_TAC std_ss [IS_INIT_REL_def, IS_TX_REL_def, IS_RX_REL_def, IS_XFER_REL_def] >>
-rw [] >>
-cheat,
-FULL_SIMP_TAC std_ss [ref_rel_def] >>
-rw [] >>
-FULL_SIMP_TAC std_ss [IS_INIT_REL_def, IS_TX_REL_def, IS_RX_REL_def, IS_XFER_REL_def] >>
-rw []]]);
+Cases_on `spi.state` >>
+rw [] >> 
+FULL_SIMP_TAC (std_ss++WORD_ss) [],
+FULL_SIMP_TAC std_ss [ref_rel_def, IS_STATE_REL_def] >>
+rw [],
+Cases_on `(0 >< 0) v: word1` >>
+FULL_SIMP_TAC (arith_ss ++ WORD_ss) [] >>
+Cases_on `n` >>
+FULL_SIMP_TAC (arith_ss++WORD_ss) [] >>
+Cases_on `n'` >>
+FULL_SIMP_TAC (arith_ss++WORD_ss) []]);
 
-(* bi-simulation: ds_abs1' exists and holds the ref_rel when driver_tau *)
+val dr_xfer_fetch_dataI_imply_abs1_xfer_fetch_data =
+store_thm("dr_xfer_fetch_dataI_imply_abs1_xfer_fetch_data",
+``!(spi:spi_state) (dr:driver_state) (ds_abs1:ds_abs1_state).
+(ref_rel ds_abs1 dr spi) /\ (dr.state = dr_xfer_fetch_dataI) ==>
+ds_abs1.state = abs1_xfer_fetch_data``,
+rw [] >>
+`IS_STATE_REL ds_abs1 dr spi` by METIS_TAC [ref_rel_def] >>
+FULL_SIMP_TAC std_ss [IS_STATE_REL_def] >>
+Cases_on `spi.state` >>
+rw [] >>
+`(dr.state <> dr_init_pre) /\
+(dr.state <> dr_init_idle) /\
+(dr.state <> dr_init_read_req) /\
+(dr.state <> dr_init_check_rep) /\
+(dr.state <> dr_init_setting) /\
+(dr.state <> dr_ready) /\
+(dr.state <> dr_tx_idle) /\
+(dr.state <> dr_tx_conf_issued) /\
+(dr.state <> dr_tx_read_txs) /\
+(dr.state <> dr_tx_check_txs) /\
+(dr.state <> dr_tx_write_data) /\
+(dr.state <> dr_tx_read_eot) /\
+(dr.state <> dr_tx_check_eot) /\
+(dr.state <> dr_tx_issue_disable) /\
+(dr.state <> dr_tx_reset_conf) /\
+(dr.state <> dr_rx_idle) /\
+(dr.state <> dr_rx_conf_issued) /\
+(dr.state <> dr_rx_read_rxs) /\
+(dr.state <> dr_rx_check_rxs) /\
+(dr.state <> dr_rx_read_rx0) /\
+(dr.state <> dr_rx_fetch_data) /\
+(dr.state <> dr_rx_issue_disable) /\
+(dr.state <> dr_rx_reset_conf) /\
+(dr.state <> dr_xfer_idle) /\
+(dr.state <> dr_xfer_conf_issued) /\
+(dr.state <> dr_xfer_read_txs) /\
+(dr.state <> dr_xfer_check_txs) /\
+(dr.state <> dr_xfer_write_dataO) /\
+(dr.state <> dr_xfer_read_rxs) /\
+(dr.state <> dr_xfer_check_rxs) /\
+(dr.state <> dr_xfer_read_rx0) /\
+(dr.state <> dr_xfer_issue_disable) /\
+(dr.state <> dr_xfer_reset_conf)` by rw [] >>
+Cases_on `ds_abs1.state` >>
+rw []);
+
+val ref_rel_check_xfer_rx0 = store_thm("ref_rel_check_xfer_rx0",
+``!(spi:spi_state) (dr:driver_state) (ds_abs1:ds_abs1_state).
+(ref_rel ds_abs1 dr spi) /\ (dr.dr_last_read_ad = SOME SPI0_RX0) /\
+(dr.dr_last_read_v = SOME v) /\ (dr.state = dr_xfer_fetch_dataI) ==>
+?ds_abs1'. (ds_abs1_tr ds_abs1 tau ds_abs1') /\ 
+(ref_rel ds_abs1' (dr_check_rx0 dr v) spi)``,
+rw [ds_abs1_tr_cases, ds_abs1_dr_tr_cases, DRIVER_ABS1_XFER_ENABLE_def] >>
+EXISTS_TAC ``driver_abs1_xfer_operations ds_abs1`` >>
+`ds_abs1.state = abs1_xfer_fetch_data` by METIS_TAC [dr_xfer_fetch_dataI_imply_abs1_xfer_fetch_data] >>
+rw [dr_check_rx0_def, driver_abs1_xfer_operations_def] >|
+[(* not the last byte*)
+`ds_abs1.ds_abs1_xfer.xfer_cur_length < (LENGTH (ds_abs1.ds_abs1_xfer.xfer_dataOUT_buffer))` by METIS_TAC [ref_rel_def] >>
+rw [driver_abs1_xfer_fetch_data_op_def] >>
+FULL_SIMP_TAC (std_ss++WORD_ss) [ref_rel_def, IS_STATE_REL_def] >>
+rw [],
+(* the last byte*)
+`~(ds_abs1.ds_abs1_xfer.xfer_cur_length < (LENGTH (ds_abs1.ds_abs1_xfer.xfer_dataOUT_buffer)))` by METIS_TAC [ref_rel_def] >>
+rw [driver_abs1_xfer_fetch_data_op_def] >>
+FULL_SIMP_TAC (std_ss++WORD_ss) [ref_rel_def, IS_STATE_REL_def] >>
+rw []]);
+
+
+(* simulation: ds_abs1' exists and holds the ref_rel when driver_tau *)
 val abs1_comb_hold_ref_rel_driver_tr = store_thm("abs1_comb_hold_ref_rel_driver_tr",
 ``!(spi:spi_state) (dr:driver_state) (ds_abs1:ds_abs1_state).
 (ref_rel ds_abs1 dr spi) /\ (driver_tr dr tau dr') ==>
 (ref_rel ds_abs1 dr' spi) \/
 (?ds_abs1'. (ds_abs1_tr ds_abs1 tau ds_abs1') /\ (ref_rel ds_abs1' dr' spi))``,
-rw [driver_tr_cases] >|
-[
-FULL_SIMP_TAC std_ss [dr_tx_syn_tr_cases] >>
+rw [driver_tr_cases] >>
+FULL_SIMP_TAC (std_ss++WORD_ss) [DR_TAU_ENABLE_def, dr_check_def] >>
 rw [] >>
-cheat,
-cheat,
-cheat,
-
-rw [dr_check_def] >>
-rw [ref_rel_check_SYSSTATUS]
-rw [ref_rel_check_CH0STAT_TX]
-rw [ref_rel_check_CH0STAT_RX]
-
-
-]);
-
+rw [ref_rel_check_sysstatus, ref_rel_check_tx_txs, ref_rel_check_tx_eot,
+ref_rel_check_rx_rxs, ref_rel_check_rx_rx0, ref_rel_check_xfer_txs,
+ref_rel_check_xfer_rxs, ref_rel_check_xfer_rx0] >>
+FULL_SIMP_TAC std_ss [ref_rel_def]);
 
 val _ = export_theory();
